tryf/Quint.State.fsti
@@ -4,13 +4,24 @@ module Quint.State
 open FStar.List.Tot
 open Quint.Rng
 open FStar.Tactics.Typeclasses
+open Quint.State.Sig
 
-[@tcclass]
-noeq type sig = {vars:eqtype; types: vars -> Type}
+module DM = FStar.DependentMap
+
+
+
 /// # State
 
+let optional #k : (k -> Type) -> k -> Type =
+  fun f v -> option (f v)
+
+// TODO Find a way to abstract implementation of this so we don't have to expose the
+// dep map impl.
 /// A state defined by a signature `sig`
-val state {| sig |} : Type
+let state {| s:sig |} = DM.t vars (optional s.types)
+
+// /// A state defined by a signature `sig`
+// val state {| sig |} : DM.t vars (optional types)
 
 /// A state initialization function
 type init_t {|sig|} = v:vars -> types v
@@ -18,14 +29,28 @@ type init_t {|sig|} = v:vars -> types v
 /// Construct a state from an initialization function
 val init : sig -> init_t -> state
 
-
+/// Predicates over states
+let is_assigned {| sig |} (m:state) k = Some? (DM.sel m k)
+let is_unassigned {| sig |} (m:state) k = None? (DM.sel m k)
+let is_fresh {| sig |} (m:state) = forall k. is_unassigned m k
+let is_updated {| sig |} (m:state) = forall k. is_assigned m k
 
 /// # State functions: the *read* effect
+
+// TODO Use `DM.restrict` to limit map to just declared variables
+// A computation of `a` that can read from `state #sig`
+// TODO Figure out how to hide and abstract these
+let state_has {|sig|} (s:state) (vs:list vars) =
+    forall v. mem v vs ==> is_assigned s v
+
+let state_not_has {|sig|} (s:state) (vs:list vars) =
+    forall v. mem v vs ==> is_unassigned s v
 
 /// A computation of a value of type `a`,
 /// over a state defined by `sig`
 /// that can read from the variables in `list vars`
-val read {|sig|} : list vars -> (a:Type) -> Type
+type read {|sig|} (vs:list vars) (a:Type)
+  = s:state{state_has s vs} -> a
 
 /// Puts a value of type `a` in a `read` context
 val pure {|sig|} #a #vs (x:a) : read vs a
@@ -61,9 +86,21 @@ val (and!) {|sig|} #a #b #vs #vs' : read vs a -> read vs' b -> read (vs @ vs') (
 
 /// # State predicates: the *action* effect
 
+/// A state predicate, i.e., an action
+///
 /// An action over the state defined by `sig`
 /// that updates the variables `vars`
-val action {|sig|} : list vars -> Type
+///
+/// - `s0` is the current state
+/// - `s` is the intermediate state to be updated (lets us ensure no state is updated twice)
+/// - `s1` is the next state specified by by the action
+type action {|sig|} (vs:list vars)
+  = s0:state{is_updated s0}
+    -> option (
+      s:state{state_not_has s vs}
+      -> s1:state{state_has s1 vs /\ (forall v. (not (mem v vs)) ==> DM.sel s1 v == DM.sel s v)}
+    )
+
 
 /// Requirements
 val req {| sig |} #vs : read vs bool -> action []
@@ -85,9 +122,8 @@ val ( |! ) {|sig|} #vs : action vs -> action vs -> action vs
 /// # Data nondetermism: the *nondet* effect
 
 /// A computation of a value of type `a` in a nondet context
-val nondet (a:Type) : Type
+type nondet (a:Type) = Rng.t a
 
-open Quint.Rng
 open Quint.Ordered
 
 module Set = Quint.Set
@@ -97,6 +133,8 @@ let run = run
 
 /// Nondeterministically select a value of type `a` from a non-empty set
 val one_of #a {|ordered a|} : Set.non_empty a -> nondet a
+
+open Quint.Rng
 
 /// Bind values in nondet contexts
 ///
@@ -116,3 +154,7 @@ val one_of #a {|ordered a|} : Set.non_empty a -> nondet a
 /// ```
 let (let?) = (let?)
 let (and?) = (and?)
+
+
+
+/// # Transitions
